theories/zoo/program_logic/prophet_multi.v
@@ -1,0 +1,627 @@
+From zoo Require Import
+  prelude.
+From zoo.common Require Import
+  function.
+From zoo.language Require Import
+  notations.
+From zoo.program_logic Require Export
+  prophet_wise.
+From zoo.diaframe Require Import
+  diaframe.
+From zoo Require Import
+  options.
+
+#[local] Program Definition prophetx prophet := {|
+  prophet_typed_strong_type :=
+    nat * prophet.(prophet_typed_strong_type) ;
+  prophet_typed_strong_of_val v1 v2 :=
+    match v2 with
+    | ValBlock _ _ [ValInt i; v2] =>
+        proph ← prophet.(prophet_typed_strong_of_val) v1 v2 ;
+        Some (₊i, proph)
+    | _ =>
+        None
+    end ;
+  prophet_typed_strong_to_val '(i, proph) :=
+    let '(v1, v2) := prophet.(prophet_typed_strong_to_val) proph in
+    (v1, (ValNat i, v2)%V)
+|}.
+Solve Obligations of prophetx with
+  try done.
+Next Obligation.
+  intros prophet (i, proph) ? ? => /=.
+  destruct (prophet.(prophet_typed_strong_to_val) proph) as (v1, v2) eqn:Heq.
+  intros [= -> ->].
+  erewrite prophet.(prophet_typed_strong_of_to_val); last done.
+  rewrite Nat2Z.id //.
+Qed.
+
+Class ProphetMultiStrongG Σ `{zoo_G : !ZooG Σ} prophet := {
+  #[local] prophet_multi_strong_G :: ProphetWiseStrongG Σ (prophetx prophet) ;
+}.
+
+Definition prophet_multi_strong_Σ prophet := #[
+  prophet_wise_strong_Σ (prophetx prophet)
+].
+#[global] Instance subG_prophet_multi_strong_Σ Σ `{zoo_G : !ZooG Σ} prophet :
+  subG (prophet_multi_strong_Σ prophet) Σ →
+  ProphetMultiStrongG Σ prophet.
+Proof.
+  solve_inG.
+Qed.
+
+Section prophet_multi_G.
+  Context (prophet : prophet_typed_strong).
+  Context `{prophet_multi_G : ProphetMultiStrongG Σ prophet}.
+
+  Notation prophetx := (
+    prophetx prophet
+  ).
+
+  Implicit Types prophs : list (prophet.(prophet_typed_strong_type)).
+  Implicit Types ipast iprophs : list (nat * prophet.(prophet_typed_strong_type)).
+  Implicit Types pasts prophss : nat → list prophet.(prophet_typed_strong_type).
+
+  Definition prophet_multi_strong_name :=
+    prophet_wise_strong_name.
+  Implicit Types γ : prophet_multi_strong_name.
+
+  #[global] Instance prophet_multi_strong_name_eq_dec : EqDecision prophet_wise_strong_name :=
+    ltac:(apply _).
+  #[global] Instance prophet_multi_strong_name_countable :
+    Countable prophet_wise_strong_name.
+  Proof.
+    apply _.
+  Qed.
+
+  #[local] Definition untangle iprophs i :=
+    (filter (λ iproph, iproph.1 = i) iprophs).*2.
+
+  #[local] Lemma untangle_cons iproph iprophs i :
+    untangle (iproph :: iprophs) i = if decide (iproph.1 = i) then [iproph.2] ++ untangle iprophs i else untangle iprophs i.
+  Proof.
+    rewrite /untangle filter_cons //.
+    case_decide; done.
+  Qed.
+  #[local] Lemma untangle_cons_True iproph iprophs i :
+    iproph.1 = i →
+    untangle (iproph :: iprophs) i = [iproph.2] ++ untangle iprophs i.
+  Proof.
+    intros <-.
+    rewrite untangle_cons decide_True //.
+  Qed.
+  #[local] Lemma untangle_cons_False iproph iprophs i :
+    iproph.1 ≠ i →
+    untangle (iproph :: iprophs) i = untangle iprophs i.
+  Proof.
+    intros Hiproph.
+    rewrite untangle_cons decide_False //.
+  Qed.
+  #[local] Lemma untangle_app iprophs1 iprophs2 i :
+    untangle (iprophs1 ++ iprophs2) i = untangle iprophs1 i ++ untangle iprophs2 i.
+  Proof.
+    rewrite /untangle filter_app fmap_app //.
+  Qed.
+  #[local] Lemma untangle_snoc iprophs iproph i :
+    untangle (iprophs ++ [iproph]) i = if decide (iproph.1 = i) then untangle iprophs i ++ [iproph.2] else untangle iprophs i.
+  Proof.
+    rewrite untangle_app /untangle filter_cons filter_nil //.
+    case_decide; rewrite ?right_id //.
+  Qed.
+  #[local] Lemma untangle_snoc_True iprophs iproph i :
+    iproph.1 = i →
+    untangle (iprophs ++ [iproph]) i = untangle iprophs i ++ [iproph.2].
+  Proof.
+    intros <-.
+    rewrite untangle_snoc decide_True //.
+  Qed.
+  #[local] Lemma untangle_snoc_False iprophs iproph i :
+    iproph.1 ≠ i →
+    untangle (iprophs ++ [iproph]) i = untangle iprophs i.
+  Proof.
+    intros Hiproph.
+    rewrite untangle_snoc decide_False //.
+  Qed.
+
+  Definition prophet_multi_strong_full γ i prophs : iProp Σ :=
+    ∃ iprophs,
+    ⌜prophs = untangle iprophs i⌝ ∗
+    prophet_wise_strong_full prophetx γ iprophs.
+  #[local] Instance : CustomIpatFormat "full" :=
+    " ( %iprophs{} &
+        -> &
+        Hfull{}
+      )
+    ".
+
+  Definition prophet_multi_strong_model pid γ pasts prophss : iProp Σ :=
+    ∃ ipast iprophs,
+    ⌜pasts ≡ᶠ untangle ipast⌝ ∗
+    ⌜prophss ≡ᶠ untangle iprophs⌝ ∗
+    prophet_wise_strong_model prophetx pid γ ipast iprophs.
+  #[local] Instance : CustomIpatFormat "model" :=
+    " ( %ipast{} &
+        %iprophs{} &
+        %Hpasts{} &
+        %Hprophss{} &
+        Hmodel{}
+      )
+    ".
+
+  Definition prophet_multi_strong_snapshot γ i past prophs : iProp Σ :=
+    ∃ ipast iprophs,
+    ⌜past = untangle ipast i⌝ ∗
+    ⌜prophs = untangle iprophs i⌝ ∗
+    prophet_wise_strong_snapshot prophetx γ ipast iprophs.
+  #[local] Instance : CustomIpatFormat "snapshot" :=
+    " ( %ipast{_{suff}} &
+        %iprophs{_{suff}} &
+        -> &
+        -> &
+        Hsnapshot
+      )
+    ".
+
+  Definition prophet_multi_strong_lb γ i lb : iProp Σ :=
+    ∃ past,
+    prophet_multi_strong_snapshot γ i past lb.
+  #[local] Instance : CustomIpatFormat "lb" :=
+    " ( %past &
+        Hsnapshot
+      )
+    ".
+
+  #[global] Instance prophet_multi_strong_full_timeless γ i prophs :
+    Timeless (prophet_multi_strong_full γ i prophs).
+  Proof.
+    apply _.
+  Qed.
+  #[global] Instance prophet_multi_strong_model_timeless pid γ pasts prophss :
+    Timeless (prophet_multi_strong_model pid γ pasts prophss).
+  Proof.
+    apply _.
+  Qed.
+  #[global] Instance prophet_multi_strong_snapshot_timeless γ i past prophs :
+    Timeless (prophet_multi_strong_snapshot γ i past prophs).
+  Proof.
+    apply _.
+  Qed.
+  #[global] Instance prophet_multi_strong_lb_timeless γ i lb :
+    Timeless (prophet_multi_strong_lb γ i lb).
+  Proof.
+    apply _.
+  Qed.
+
+  #[global] Instance prophet_multi_strong_full_persistent γ i prophs :
+    Persistent (prophet_multi_strong_full γ i prophs).
+  Proof.
+    apply _.
+  Qed.
+  #[global] Instance prophet_multi_strong_snapshot_persistent γ i past prophs :
+    Persistent (prophet_multi_strong_snapshot γ i past prophs).
+  Proof.
+    apply _.
+  Qed.
+  #[global] Instance prophet_multi_strong_lb_persistent γ i lb :
+    Persistent (prophet_multi_strong_lb γ i lb).
+  Proof.
+    apply _.
+  Qed.
+
+  Lemma prophet_multi_strong_model_exclusive pid γ1 pasts1 prophss1 γ2 pasts2 prophss2 :
+    prophet_multi_strong_model pid γ1 pasts1 prophss1 -∗
+    prophet_multi_strong_model pid γ2 pasts2 prophss2 -∗
+    False.
+  Proof.
+    iIntros "(:model =1) (:model =2)".
+    iApply (prophet_wise_strong_model_exclusive with "Hmodel1 Hmodel2").
+  Qed.
+
+  Lemma prophet_multi_strong_full_get {pid γ pasts prophss} i :
+    prophet_multi_strong_model pid γ pasts prophss ⊢
+    prophet_multi_strong_full γ i (pasts i ++ prophss i).
+  Proof.
+    iIntros "(:model)".
+    iDestruct (prophet_wise_strong_full_get with "Hmodel") as "$".
+    rewrite Hpasts Hprophss untangle_app //.
+  Qed.
+  Lemma prophet_multi_strong_full_get' {pid γ pasts prophss} i :
+    prophet_multi_strong_model pid γ pasts prophss ⊢
+      ∃ prophs,
+      prophet_multi_strong_full γ i prophs.
+  Proof.
+    rewrite prophet_multi_strong_full_get. iSteps.
+  Qed.
+  Lemma prophet_multi_strong_full_valid pid γ pasts prophss i prophs :
+    prophet_multi_strong_model pid γ pasts prophss -∗
+    prophet_multi_strong_full γ i prophs -∗
+    ⌜prophs = pasts i ++ prophss i⌝.
+  Proof.
+    iIntros "(:model =1) (:full =2)". simplify.
+    iDestruct (prophet_wise_strong_full_valid with "Hmodel1 Hfull2") as %->.
+    rewrite Hpasts1 Hprophss1 untangle_app //.
+  Qed.
+  Lemma prophet_multi_strong_full_agree γ i prophs1 prophs2 :
+    prophet_multi_strong_full γ i prophs1 -∗
+    prophet_multi_strong_full γ i prophs2 -∗
+    ⌜prophs1 = prophs2⌝.
+  Proof.
+    iIntros "(:full =1) (:full =2)". simplify.
+    iDestruct (prophet_wise_strong_full_agree with "Hfull1 Hfull2") as %->.
+    iSteps.
+  Qed.
+
+  Lemma prophet_multi_strong_snapshot_get {pid γ pasts prophss} i :
+    prophet_multi_strong_model pid γ pasts prophss ⊢
+    prophet_multi_strong_snapshot γ i (pasts i) (prophss i).
+  Proof.
+    iIntros "(:model)".
+    iDestruct (prophet_wise_strong_snapshot_get with "Hmodel") as "$".
+    iSteps.
+  Qed.
+  Lemma prophet_multi_strong_snapshot_valid pid γ pasts prophss i past prophs :
+    prophet_multi_strong_model pid γ pasts prophss -∗
+    prophet_multi_strong_snapshot γ i past prophs -∗
+      ∃ past',
+      ⌜pasts i = past ++ past'⌝ ∗
+      ⌜prophs = past' ++ prophss i⌝.
+  Proof.
+    iIntros "(:model) (:snapshot suff=)".
+    iDestruct (prophet_wise_strong_snapshot_valid with "Hmodel Hsnapshot") as "(%ipast' & -> & ->)".
+    iExists (untangle ipast' i). iSplit; iPureIntro.
+    all: rewrite ?Hpasts ?Hprophss untangle_app //.
+  Qed.
+
+  Lemma prophet_multi_strong_lb_get {pid γ pasts prophss} i :
+    prophet_multi_strong_model pid γ pasts prophss ⊢
+    prophet_multi_strong_lb γ i (prophss i).
+  Proof.
+    rewrite (prophet_multi_strong_snapshot_get i).
+    iIntros "Hsnapshot".
+    iExists _. iFrame.
+  Qed.
+  Lemma prophet_multi_strong_lb_valid pid γ pasts prophss i lb :
+    prophet_multi_strong_model pid γ pasts prophss -∗
+    prophet_multi_strong_lb γ i lb -∗
+      ∃ past1 past2,
+      ⌜pasts i = past1 ++ past2⌝ ∗
+      ⌜lb = past2 ++ prophss i⌝.
+  Proof.
+    iIntros "Hmodel (:lb)".
+    iExists past.
+    iApply (prophet_multi_strong_snapshot_valid with "Hmodel Hsnapshot").
+  Qed.
+
+  Lemma prophet_multi_strong_wp_proph E :
+    {{{
+      True
+    }}}
+      Proph @ E
+    {{{ pid γ prophss,
+      RET #pid;
+      prophet_multi_strong_model pid γ (λ _, []) prophss
+    }}}.
+  Proof.
+    iIntros "%Φ _ HΦ".
+    wp_apply (prophet_wise_strong_wp_proph prophetx with "[//]") as (pid γ iprophs) "Hmodel".
+    iApply "HΦ".
+    iExists [], iprophs. rewrite /funeq. iSteps.
+  Qed.
+
+  Lemma prophet_multi_strong_wp_resolve e pid i v γ pasts prophss E Φ :
+    Atomic e →
+    to_val e = None →
+    (0 ≤ i)%Z →
+    prophet_multi_strong_model pid γ pasts prophss -∗
+    WP e @ E {{ w,
+      ∃ proph,
+      ⌜(w, v) = prophet.(prophet_typed_strong_to_val) proph⌝ ∗
+        ∀ prophs,
+        ⌜prophss ₊i = proph :: prophs⌝ -∗
+        prophet_multi_strong_model pid γ (alter (.++ [proph]) ₊i pasts) (<[₊i := prophs]> prophss) -∗
+        Φ w
+    }} -∗
+    WP Resolve e #pid (#i, v)%V @ E {{ Φ }}.
+  Proof.
+    iIntros "% % %Hi (:model) HΦ".
+    Z_to_nat i. rewrite Nat2Z.id.
+    wp_apply (prophet_wise_strong_wp_resolve with "Hmodel"); first done.
+    wp_apply (wp_wand with "HΦ") as (w) "(%proph & %Hproph & HΦ)".
+    iExists (i, proph). iSplit.
+    - iPureIntro. rewrite /= -Hproph //.
+    - iIntros "%iprophs' -> Hmodel".
+      iApply ("HΦ" $! (untangle iprophs' i)).
+      + iPureIntro. rewrite Hprophss untangle_cons_True //.
+      + iExists _, _. iFrame. iSplit; iPureIntro; intros j.
+        * rewrite function.fn_lookup_alter untangle_snoc Hpasts /=.
+          case_decide; subst; done.
+        * rewrite function.fn_lookup_insert Hprophss untangle_cons /=.
+          case_decide; subst; done.
+  Qed.
+  Lemma prophet_multi_strong_wp_resolve' e pid i v γ pasts prophss E Φ :
+    Atomic e →
+    to_val e = None →
+    prophet_multi_strong_model pid γ pasts prophss -∗
+    WP e @ E {{ w,
+      ∃ proph,
+      ⌜(w, v) = prophet.(prophet_typed_strong_to_val) proph⌝ ∗
+        ∀ prophs,
+        ⌜prophss i = proph :: prophs⌝ -∗
+        prophet_multi_strong_model pid γ (alter (.++ [proph]) i pasts) (<[i := prophs]> prophss) -∗
+        Φ w
+    }} -∗
+    WP Resolve e #pid (#i, v)%V @ E {{ Φ }}.
+  Proof.
+    iIntros "% % Hmodel HΦ".
+    iApply (prophet_multi_strong_wp_resolve with "Hmodel"); [done | lia |].
+    rewrite Nat2Z.id. iSteps.
+  Qed.
+End prophet_multi_G.
+
+#[global] Opaque prophet_multi_strong_name.
+#[global] Opaque prophet_multi_strong_full.
+#[global] Opaque prophet_multi_strong_model.
+#[global] Opaque prophet_multi_strong_snapshot.
+#[global] Opaque prophet_multi_strong_lb.
+
+Class ProphetMultiG Σ `{zoo_G : !ZooG Σ} prophet := {
+  #[local] prophet_multi_G :: ProphetMultiStrongG Σ prophet ;
+}.
+
+Definition prophet_multi_Σ prophet := #[
+  prophet_multi_strong_Σ prophet
+].
+#[global] Instance subG_prophet_multi_Σ Σ `{zoo_G : !ZooG Σ} prophet :
+  subG (prophet_multi_Σ prophet) Σ →
+  ProphetMultiG Σ prophet.
+Proof.
+  solve_inG.
+Qed.
+
+Section prophet_multi_G.
+  Context (prophet : prophet_typed).
+  Context `{prophet_multi_G : ProphetMultiG Σ prophet}.
+
+  Implicit Types spasts sprophss : nat → list (val * prophet.(prophet_typed_type)).
+
+  Definition prophet_multi_name :=
+    prophet_multi_strong_name.
+  Implicit Types γ : prophet_multi_name.
+
+  Definition prophet_multi_full γ i prophs : iProp Σ :=
+    ∃ sprophs,
+    ⌜prophs = sprophs.*2⌝ ∗
+    prophet_multi_strong_full prophet γ i sprophs.
+  #[local] Instance : CustomIpatFormat "full" :=
+    " ( %sprophs{} &
+        -> &
+        Hfull{}
+      )
+    ".
+
+  Definition prophet_multi_model pid γ pasts prophss : iProp Σ :=
+    ∃ spasts sprophss,
+    ⌜pasts ≡ᶠ fmap snd ∘ spasts⌝ ∗
+    ⌜prophss ≡ᶠ fmap snd ∘ sprophss⌝ ∗
+    prophet_multi_strong_model prophet pid γ spasts sprophss.
+  #[local] Instance : CustomIpatFormat "model" :=
+    " ( %spasts{} &
+        %sprophss{} &
+        %Hpasts{} &
+        %Hprophss{} &
+        Hmodel{}
+      )
+    ".
+
+  Definition prophet_multi_snapshot γ i past prophs : iProp Σ :=
+    ∃ spast sprophs,
+    ⌜past = spast.*2⌝ ∗
+    ⌜prophs = sprophs.*2⌝ ∗
+    prophet_multi_strong_snapshot prophet γ i spast sprophs.
+  #[local] Instance : CustomIpatFormat "snapshot" :=
+    " ( %spast{} &
+        %sprophs{} &
+        -> &
+        -> &
+        Hsnapshot
+      )
+    ".
+
+  Definition prophet_multi_lb γ i lb : iProp Σ :=
+    ∃ slb,
+    ⌜lb = slb.*2⌝ ∗
+    prophet_multi_strong_lb prophet γ i slb.
+  #[local] Instance : CustomIpatFormat "lb" :=
+    " ( %slb &
+        -> &
+        Hlb
+      )
+    ".
+
+  #[global] Instance prophet_multi_full_timeless γ i prophs :
+    Timeless (prophet_multi_full γ i prophs).
+  Proof.
+    apply _.
+  Qed.
+  #[global] Instance prophet_multi_model_timeless pid γ pasts prophss :
+    Timeless (prophet_multi_model pid γ pasts prophss).
+  Proof.
+    apply _.
+  Qed.
+  #[global] Instance prophet_multi_snapshot_timeless γ i past prophs :
+    Timeless (prophet_multi_snapshot γ i past prophs).
+  Proof.
+    apply _.
+  Qed.
+  #[global] Instance prophet_multi_lb_timeless γ i lb :
+    Timeless (prophet_multi_lb γ i lb).
+  Proof.
+    apply _.
+  Qed.
+  #[global] Instance prophet_multi_full_persistent γ i prophs :
+    Persistent (prophet_multi_full γ i prophs).
+  Proof.
+    apply _.
+  Qed.
+  #[global] Instance prophet_multi_snapshot_persistent γ i past prophs :
+    Persistent (prophet_multi_snapshot γ i past prophs).
+  Proof.
+    apply _.
+  Qed.
+  #[global] Instance prophet_multi_lb_persistent γ i lb :
+    Persistent (prophet_multi_lb γ i lb).
+  Proof.
+    apply _.
+  Qed.
+
+  Lemma prophet_multi_model_exclusive pid γ1 pasts1 prophss1 γ2 pasts2 prophss2 :
+    prophet_multi_model pid γ1 pasts1 prophss1 -∗
+    prophet_multi_model pid γ2 pasts2 prophss2 -∗
+    False.
+  Proof.
+    iIntros "(:model =1) (:model =2)".
+    iApply (prophet_multi_strong_model_exclusive with "Hmodel1 Hmodel2").
+  Qed.
+
+  Lemma prophet_multi_full_get {pid γ pasts prophss} i :
+    prophet_multi_model pid γ pasts prophss ⊢
+    prophet_multi_full γ i (pasts i ++ prophss i).
+  Proof.
+    iIntros "(:model)".
+    iDestruct (prophet_multi_strong_full_get with "Hmodel") as "$".
+    rewrite Hpasts Hprophss fmap_app //.
+  Qed.
+  Lemma prophet_multi_full_get' {pid γ pasts prophss} i :
+    prophet_multi_model pid γ pasts prophss ⊢
+      ∃ prophs,
+      prophet_multi_full γ i prophs.
+  Proof.
+    rewrite prophet_multi_full_get. iSteps.
+  Qed.
+  Lemma prophet_multi_full_valid pid γ pasts prophss i prophs :
+    prophet_multi_model pid γ pasts prophss -∗
+    prophet_multi_full γ i prophs -∗
+    ⌜prophs = pasts i ++ prophss i⌝.
+  Proof.
+    iIntros "(:model =1) (:full =2)". simplify.
+    iDestruct (prophet_multi_strong_full_valid with "Hmodel1 Hfull2") as %->.
+    rewrite Hpasts1 Hprophss1 fmap_app //.
+  Qed.
+  Lemma prophet_multi_full_agree γ i prophs1 prophs2 :
+    prophet_multi_full γ i prophs1 -∗
+    prophet_multi_full γ i prophs2 -∗
+    ⌜prophs1 = prophs2⌝.
+  Proof.
+    iIntros "(:full =1) (:full =2)". simplify.
+    iDestruct (prophet_multi_strong_full_agree with "Hfull1 Hfull2") as %->.
+    iSteps.
+  Qed.
+
+  Lemma prophet_multi_snapshot_get {pid γ pasts prophss} i :
+    prophet_multi_model pid γ pasts prophss ⊢
+    prophet_multi_snapshot γ i (pasts i) (prophss i).
+  Proof.
+    iIntros "(:model)".
+    iSteps.
+    iApply (prophet_multi_strong_snapshot_get with "Hmodel").
+  Qed.
+  Lemma prophet_multi_snapshot_valid pid γ pasts prophss i past prophs :
+    prophet_multi_model pid γ pasts prophss -∗
+    prophet_multi_snapshot γ i past prophs -∗
+      ∃ past',
+      ⌜pasts i = past ++ past'⌝ ∗
+      ⌜prophs = past' ++ prophss i⌝.
+  Proof.
+    iIntros "(:model) (:snapshot =')".
+    iDestruct (prophet_multi_strong_snapshot_valid with "Hmodel Hsnapshot") as "(%spast'' & %Heq & ->)".
+    iExists spast''.*2. iSplit; iPureIntro.
+    all: rewrite ?Hpasts ?Hprophss /= ?Heq fmap_app //.
+  Qed.
+
+  Lemma prophet_multi_lb_get {pid γ pasts prophss} i :
+    prophet_multi_model pid γ pasts prophss -∗
+    prophet_multi_lb γ i (prophss i).
+  Proof.
+    iIntros "(:model)".
+    iStep.
+    iApply (prophet_multi_strong_lb_get with "Hmodel").
+  Qed.
+  Lemma prophet_multi_lb_valid pid γ pasts prophss i lb :
+    prophet_multi_model pid γ pasts prophss -∗
+    prophet_multi_lb γ i lb -∗
+      ∃ past1 past2,
+      ⌜pasts i = past1 ++ past2⌝ ∗
+      ⌜lb = past2 ++ prophss i⌝.
+  Proof.
+    iIntros "(:model) (:lb)".
+    iDestruct (prophet_multi_strong_lb_valid with "Hmodel Hlb") as "(%spast1 & %spast2 & %Heq & ->)".
+    iExists spast1.*2, spast2.*2. iSplit; iPureIntro.
+    all: rewrite ?Hpasts ?Hprophss /= ?Heq fmap_app //.
+  Qed.
+
+  Lemma prophet_multi_wp_proph E :
+    {{{
+      True
+    }}}
+      Proph @ E
+    {{{ pid γ prophss,
+      RET #pid;
+      prophet_multi_model pid γ (λ _, []) prophss
+    }}}.
+  Proof.
+    iIntros "%Φ _ HΦ".
+    wp_apply (prophet_multi_strong_wp_proph prophet with "[//]") as "%pid %γ %sprophss Hmodel".
+    iApply "HΦ".
+    iExists (λ _, []), sprophss. rewrite /funeq. iSteps.
+  Qed.
+
+  Lemma prophet_multi_wp_resolve proph e pid i v γ pasts prophss E Φ :
+    Atomic e →
+    to_val e = None →
+    (0 ≤ i)%Z →
+    v = prophet.(prophet_typed_to_val) proph →
+    prophet_multi_model pid γ pasts prophss -∗
+    WP e @ E {{ w,
+      ∀ prophs,
+      ⌜prophss ₊i = proph :: prophs⌝ -∗
+      prophet_multi_model pid γ (alter (.++ [proph]) ₊i pasts) (<[₊i := prophs]> prophss) -∗
+      Φ w
+    }} -∗
+    WP Resolve e #pid (#i, v)%V @ E {{ Φ }}.
+  Proof.
+    iIntros (? ? Hi ->) "(:model) HΦ".
+    wp_apply (prophet_multi_strong_wp_resolve with "Hmodel"); [done.. |].
+    wp_apply (wp_wand with "HΦ") as "%w HΦ".
+    iExists (w, proph). iStep. iIntros "%sprophs %Heq Hmodel".
+    iApply ("HΦ" with "[%]").
+    { rewrite Hprophss /= Heq //. }
+    iExists _, _. iFrame. iSplit; iPureIntro; intros j.
+    - rewrite /= !function.fn_lookup_alter /=.
+      case_decide; last done. rewrite fmap_app Hpasts //.
+    - rewrite /= !function.fn_lookup_insert /=.
+      case_decide; done.
+  Qed.
+  Lemma prophet_multi_wp_resolve' proph e pid i v γ pasts prophss E Φ :
+    Atomic e →
+    to_val e = None →
+    v = prophet.(prophet_typed_to_val) proph →
+    prophet_multi_model pid γ pasts prophss -∗
+    WP e @ E {{ w,
+      ∀ prophs,
+      ⌜prophss i = proph :: prophs⌝ -∗
+      prophet_multi_model pid γ (alter (.++ [proph]) i pasts) (<[i := prophs]> prophss) -∗
+      Φ w
+    }} -∗
+    WP Resolve e #pid (#i, v)%V @ E {{ Φ }}.
+  Proof.
+    iIntros "% % % Hmodel HΦ".
+    iApply (prophet_multi_wp_resolve with "Hmodel"); [done | lia | done |].
+    rewrite Nat2Z.id. iSteps.
+  Qed.
+End prophet_multi_G.
+
+#[global] Opaque prophet_multi_name.
+#[global] Opaque prophet_multi_full.
+#[global] Opaque prophet_multi_model.
+#[global] Opaque prophet_multi_snapshot.
+#[global] Opaque prophet_multi_lb.
