theories/zoo/program_logic/prophet_typed.v
@@ -1,0 +1,386 @@
+From zoo Require Import
+  prelude.
+From zoo.language Require Import
+  notations.
+From zoo.program_logic Require Export
+  wp.
+From zoo.diaframe Require Import
+  diaframe.
+From zoo Require Import
+  options.
+
+Record prophet_typed_strong := {
+  prophet_typed_strong_type : Type ;
+  prophet_typed_strong_of_val : val → val → option prophet_typed_strong_type ;
+  prophet_typed_strong_to_val : prophet_typed_strong_type → val * val ;
+
+  prophet_typed_strong_of_to_val proph w v :
+    (w, v) = prophet_typed_strong_to_val proph →
+    prophet_typed_strong_of_val w v = Some proph ;
+}.
+#[global] Arguments Build_prophet_typed_strong {_ _ _} _ : assert.
+
+Section prophet_typed_strong.
+  Context (prophet : prophet_typed_strong).
+  Context `{zoo_G : !ZooG Σ}.
+
+  #[local] Fixpoint prophet_typed_strong_process prophs :=
+    match prophs with
+    | [] =>
+        []
+    | (w, v) :: prophs =>
+        match prophet.(prophet_typed_strong_of_val) w v with
+        | None =>
+            []
+        | Some proph =>
+            proph :: prophet_typed_strong_process prophs
+        end
+    end.
+  Definition prophet_typed_strong_model pid prophs : iProp Σ :=
+    ∃ uprophs,
+    ⌜prophs = prophet_typed_strong_process uprophs⌝ ∗
+    prophet_model' pid uprophs.
+  #[local] Instance : CustomIpatFormat "model" :=
+    " ( %uprophs &
+        %Hprophs &
+        Hpid
+      )
+    ".
+
+  #[global] Instance prophet_typed_strong_model_timeless pid prophs :
+    Timeless (prophet_typed_strong_model pid prophs).
+  Proof.
+    apply _.
+  Qed.
+
+  Lemma prophet_typed_strong_model_exclusive pid prophs1 prophs2 :
+    prophet_typed_strong_model pid prophs1 -∗
+    prophet_typed_strong_model pid prophs2 -∗
+    False.
+  Proof.
+    iSteps.
+  Qed.
+
+  Lemma prophet_typed_strong_wp_proph E :
+    {{{
+      True
+    }}}
+      Proph @ E
+    {{{ pid prophs,
+      RET #pid;
+      prophet_typed_strong_model pid prophs
+    }}}.
+  Proof.
+    iIntros "%Φ _ HΦ".
+    wp_apply (wp_proph with "[//]").
+    iSteps.
+  Qed.
+
+  Lemma prophet_typed_strong_wp_resolve e pid v prophs E Φ :
+    Atomic e →
+    to_val e = None →
+    prophet_typed_strong_model pid prophs -∗
+    WP e @ E {{ w,
+      ∃ proph,
+      ⌜(w, v) = prophet.(prophet_typed_strong_to_val) proph⌝ ∗
+        ∀ prophs',
+        ⌜prophs = proph :: prophs'⌝ -∗
+        prophet_typed_strong_model pid prophs' -∗
+        Φ w
+    }} -∗
+    WP Resolve e #pid v @ E {{ Φ }}.
+  Proof.
+    iIntros "% % (:model) HΦ".
+    wp_apply (wp_resolve with "Hpid"); first done.
+    wp_apply (wp_wand with "HΦ") as "%w (%proph & % & HΦ) %prophs' -> Hpid".
+    rewrite /= (prophet_typed_strong_of_to_val _ proph) // in Hprophs.
+    iSteps.
+  Qed.
+End prophet_typed_strong.
+
+#[global] Opaque prophet_typed_strong_model.
+
+Record prophet_typed_strong_1 := {
+  prophet_typed_strong_1_type : Type ;
+  prophet_typed_strong_1_of_val : val → val → option prophet_typed_strong_1_type ;
+  prophet_typed_strong_1_to_val : prophet_typed_strong_1_type → val * val ;
+
+  #[global] prophet_typed_strong_1_type_inhabited ::
+    Inhabited prophet_typed_strong_1_type ;
+
+  prophet_typed_strong_1_of_to_val proph w v :
+    (w, v) = prophet_typed_strong_1_to_val proph →
+    prophet_typed_strong_1_of_val w v = Some proph ;
+}.
+#[global] Arguments Build_prophet_typed_strong_1 {_ _ _ _} _ : assert.
+
+Section prophet_typed_strong_1.
+  Context (prophet : prophet_typed_strong_1).
+  Context `{zoo_G : !ZooG Σ}.
+
+  Program Definition prophet_typed_strong_1_to_prophet := {|
+    prophet_typed_strong_type :=
+      prophet.(prophet_typed_strong_1_type) ;
+    prophet_typed_strong_of_val :=
+      prophet.(prophet_typed_strong_1_of_val) ;
+    prophet_typed_strong_to_val :=
+      prophet.(prophet_typed_strong_1_to_val) ;
+  |}.
+  Next Obligation.
+    apply prophet_typed_strong_1_of_to_val.
+  Qed.
+
+  Definition prophet_typed_strong_1_model pid proph : iProp Σ :=
+    ∃ prophs,
+    prophet_typed_strong_model prophet_typed_strong_1_to_prophet pid prophs ∗
+    ⌜if prophs is proph' :: _ then proph' = proph else True⌝.
+  #[local] Instance : CustomIpatFormat "model" :=
+    " ( %prophs{} &
+        Hmodel{} &
+        %
+      )
+    ".
+
+  #[global] Instance prophet_typed_strong_1_model_timeless pid proph :
+    Timeless (prophet_typed_strong_1_model pid proph).
+  Proof.
+    apply _.
+  Qed.
+
+  Lemma prophet_typed_strong_1_model_exclusive pid proph1 proph2 :
+    prophet_typed_strong_1_model pid proph1 -∗
+    prophet_typed_strong_1_model pid proph2 -∗
+    False.
+  Proof.
+    iIntros "(:model =1) (:model =2)".
+    iApply (prophet_typed_strong_model_exclusive with "Hmodel1 Hmodel2").
+  Qed.
+
+  Lemma prophet_typed_strong_1_wp_proph E :
+    {{{
+      True
+    }}}
+      Proph @ E
+    {{{ pid proph,
+      RET #pid;
+      prophet_typed_strong_1_model pid proph
+    }}}.
+  Proof.
+    iIntros "%Φ _ HΦ".
+    wp_apply (prophet_typed_strong_wp_proph with "[//]") as "%pid %prophs Hmodel".
+    destruct prophs as [| proph prophs'] eqn:Heq.
+    1: iApply ("HΦ" $! pid inhabitant).
+    2: iApply ("HΦ" $! pid proph).
+    all: iSteps.
+  Qed.
+
+  Lemma prophet_typed_strong_1_wp_resolve e pid v proph E Φ :
+    Atomic e →
+    to_val e = None →
+    prophet_typed_strong_1_model pid proph -∗
+    WP e @ E {{ w,
+      ∃ proph',
+      ⌜(w, v) = prophet.(prophet_typed_strong_1_to_val) proph'⌝ ∗
+      (⌜proph = proph'⌝ -∗ Φ w)
+    }} -∗
+    WP Resolve e #pid v @ E {{ Φ }}.
+  Proof.
+    iIntros (? ?) "(:model) HΦ".
+    wp_apply (prophet_typed_strong_wp_resolve with "Hmodel"); first done.
+    iSteps.
+  Qed.
+End prophet_typed_strong_1.
+
+#[global] Opaque prophet_typed_strong_1_model.
+
+Coercion prophet_typed_strong_1_to_prophet : prophet_typed_strong_1 >-> prophet_typed_strong.
+
+Record prophet_typed := {
+  prophet_typed_type : Type ;
+  prophet_typed_of_val : val → option prophet_typed_type ;
+  prophet_typed_to_val : prophet_typed_type → val ;
+
+  prophet_typed_of_to_val proph v :
+    v = prophet_typed_to_val proph →
+    prophet_typed_of_val v = Some proph ;
+}.
+#[global] Arguments Build_prophet_typed {_ _ _} _ : assert.
+
+Section prophet_typed.
+  Context (prophet : prophet_typed).
+  Context `{zoo_G : !ZooG Σ}.
+
+  Program Definition prophet_typed_to_strong := {|
+    prophet_typed_strong_type :=
+      val * prophet.(prophet_typed_type) ;
+    prophet_typed_strong_of_val w v :=
+      match prophet.(prophet_typed_of_val) v with
+      | None =>
+          None
+      | Some proph =>
+          Some (w, proph)
+      end ;
+    prophet_typed_strong_to_val '(w, proph) :=
+      (w, prophet.(prophet_typed_to_val) proph) ;
+  |}.
+  Next Obligation.
+    intros (w & proph) _w v [= -> ->].
+    erewrite prophet_typed_of_to_val => //.
+  Qed.
+
+  Definition prophet_typed_model pid prophs : iProp Σ :=
+    ∃ sprophs,
+    ⌜prophs = sprophs.*2⌝ ∗
+    prophet_typed_strong_model prophet_typed_to_strong pid sprophs.
+  #[local] Instance : CustomIpatFormat "model" :=
+    " ( %sprophs{} &
+        -> &
+        Hmodel{}
+      )
+    ".
+
+  #[global] Instance prophet_typed_model_timeless pid prophs :
+    Timeless (prophet_typed_model pid prophs).
+  Proof.
+    apply _.
+  Qed.
+
+  Lemma prophet_typed_model_exclusive pid prophs1 prophs2 :
+    prophet_typed_model pid prophs1 -∗
+    prophet_typed_model pid prophs2 -∗
+    False.
+  Proof.
+    iIntros "(:model =1) (:model =2)".
+    iApply (prophet_typed_strong_model_exclusive with "Hmodel1 Hmodel2").
+  Qed.
+
+  Lemma prophet_typed_wp_proph E :
+    {{{
+      True
+    }}}
+      Proph @ E
+    {{{ pid prophs,
+      RET #pid;
+      prophet_typed_model pid prophs
+    }}}.
+  Proof.
+    iIntros "%Φ _ HΦ".
+    wp_apply (prophet_typed_strong_wp_proph with "[//]").
+    iSteps. done.
+  Qed.
+
+  Lemma prophet_typed_wp_resolve proph e pid v prophs E Φ :
+    Atomic e →
+    to_val e = None →
+    v = prophet.(prophet_typed_to_val) proph →
+    prophet_typed_model pid prophs -∗
+    WP e @ E {{ w,
+      ∀ prophs',
+      ⌜prophs = proph :: prophs'⌝ -∗
+      prophet_typed_model pid prophs' -∗
+      Φ w
+    }} -∗
+    WP Resolve e #pid v @ E {{ Φ }}.
+  Proof.
+    iIntros (? ? ->) "(:model) HΦ".
+    wp_apply (prophet_typed_strong_wp_resolve with "Hmodel"); first done.
+    wp_apply (wp_wand with "HΦ") as "%w HΦ".
+    iExists (w, proph). iSteps.
+  Qed.
+End prophet_typed.
+
+#[global] Opaque prophet_typed_model.
+
+Coercion prophet_typed_to_strong : prophet_typed >-> prophet_typed_strong.
+
+Record prophet_typed_1 := {
+  prophet_typed_1_type : Type ;
+  prophet_typed_1_of_val : val → option prophet_typed_1_type ;
+  prophet_typed_1_to_val : prophet_typed_1_type → val ;
+
+  #[global] prophet_typed_1_type_inhabited ::
+    Inhabited prophet_typed_1_type ;
+
+  prophet_typed_1_of_to_val proph v :
+    v = prophet_typed_1_to_val proph →
+    prophet_typed_1_of_val v = Some proph ;
+}.
+#[global] Arguments Build_prophet_typed_1 {_ _ _ _} _ : assert.
+
+Section prophet_typed_1.
+  Context (prophet : prophet_typed_1).
+  Context `{zoo_G : !ZooG Σ}.
+
+  Program Definition prophet_typed_1_to_prophet := {|
+    prophet_typed_type :=
+      prophet.(prophet_typed_1_type) ;
+    prophet_typed_of_val :=
+      prophet.(prophet_typed_1_of_val) ;
+    prophet_typed_to_val :=
+      prophet.(prophet_typed_1_to_val) ;
+  |}.
+  Next Obligation.
+    apply prophet_typed_1_of_to_val.
+  Qed.
+
+  Definition prophet_typed_1_model pid proph : iProp Σ :=
+    ∃ prophs,
+    prophet_typed_model prophet_typed_1_to_prophet pid prophs ∗
+    ⌜if prophs is proph' :: _ then proph' = proph else True⌝.
+  #[local] Instance : CustomIpatFormat "model" :=
+    " ( %prophs{} &
+        Hmodel{} &
+        %
+      )
+    ".
+
+  #[global] Instance prophet_typed_1_model_timeless pid proph :
+    Timeless (prophet_typed_1_model pid proph).
+  Proof.
+    apply _.
+  Qed.
+
+  Lemma prophet_typed_1_model_exclusive pid proph1 proph2 :
+    prophet_typed_1_model pid proph1 -∗
+    prophet_typed_1_model pid proph2 -∗
+    False.
+  Proof.
+    iIntros "(:model =1) (:model =2)".
+    iApply (prophet_typed_model_exclusive with "Hmodel1 Hmodel2").
+  Qed.
+
+  Lemma prophet_typed_1_wp_proph E :
+    {{{
+      True
+    }}}
+      Proph @ E
+    {{{ pid proph,
+      RET #pid;
+      prophet_typed_1_model pid proph
+    }}}.
+  Proof.
+    iIntros "%Φ _ HΦ".
+    wp_apply (prophet_typed_wp_proph with "[//]") as "%pid %prophs Hmodel".
+    destruct prophs as [| proph prophs'] eqn:Heq.
+    1: iApply ("HΦ" $! pid inhabitant).
+    2: iApply ("HΦ" $! pid proph).
+    all: iSteps.
+  Qed.
+
+  Lemma prophet_typed_1_wp_resolve proph e pid v proph' E Φ :
+    Atomic e →
+    to_val e = None →
+    v = prophet.(prophet_typed_1_to_val) proph →
+    prophet_typed_1_model pid proph' -∗
+    WP e @ E {{ w, ⌜proph' = proph⌝ -∗ Φ w }} -∗
+    WP Resolve e #pid v @ E {{ Φ }}.
+  Proof.
+    iIntros (? ? ->) "(:model) HΦ".
+    wp_apply (prophet_typed_wp_resolve with "Hmodel"); [done.. |].
+    iSteps.
+  Qed.
+End prophet_typed_1.
+
+#[global] Opaque prophet_typed_1_model.
+
+Coercion prophet_typed_1_to_prophet : prophet_typed_1 >-> prophet_typed.
