theories/zoo/program_logic/prophet_wise.v
@@ -1,0 +1,486 @@
+From zoo Require Import
+  prelude.
+From zoo.common Require Import
+  countable.
+From zoo.iris.base_logic Require Import
+  lib.agree
+  lib.mono_list.
+From zoo.language Require Import
+  notations.
+From zoo.program_logic Require Export
+  prophet_typed.
+From zoo.diaframe Require Import
+  diaframe.
+From zoo Require Import
+  options.
+
+Class ProphetWiseStrongG Σ `{zoo_G : !ZooG Σ} prophet := {
+  #[local] prophet_wise_strong_G_full_G :: AgreeG Σ (leibnizO (list prophet.(prophet_typed_strong_type))) ;
+  #[local] prophet_wise_strong_G_past_G :: MonoListG Σ prophet.(prophet_typed_strong_type) ;
+}.
+
+Definition prophet_wise_strong_Σ prophet := #[
+  agree_Σ (leibnizO (list prophet.(prophet_typed_strong_type))) ;
+  mono_list_Σ prophet.(prophet_typed_strong_type)
+].
+#[global] Instance subG_prophet_wise_strong_Σ Σ `{zoo_G : !ZooG Σ} prophet :
+  subG (prophet_wise_strong_Σ prophet) Σ →
+  ProphetWiseStrongG Σ prophet.
+Proof.
+  solve_inG.
+Qed.
+
+Section prophet_wise_G.
+  Context (prophet : prophet_typed_strong).
+  Context `{prophet_wise_G : ProphetWiseStrongG Σ prophet}.
+
+  Record prophet_wise_strong_name := {
+    prophet_wise_strong_name_full : gname ;
+    prophet_wise_strong_name_past : gname ;
+  }.
+
+  #[global] Instance prophet_wise_strong_name_eq_dec : EqDecision prophet_wise_strong_name :=
+    ltac:(solve_decision).
+  #[global] Instance prophet_wise_strong_name_countable :
+    Countable prophet_wise_strong_name.
+  Proof.
+    solve_countable.
+  Qed.
+
+  Definition prophet_wise_strong_full γ prophs : iProp Σ :=
+    agree_on γ.(prophet_wise_strong_name_full) prophs.
+  #[local] Instance : CustomIpatFormat "full" :=
+    "#Hfull{}".
+
+  Definition prophet_wise_strong_model pid γ past prophs : iProp Σ :=
+    prophet_wise_strong_full γ (past ++ prophs) ∗
+    mono_list_auth γ.(prophet_wise_strong_name_past) (DfracOwn 1) past ∗
+    prophet_typed_strong_model prophet pid prophs.
+  #[local] Instance : CustomIpatFormat "model" :=
+    " ( #Hfull{} &
+        Hpast{}_auth &
+        Hmodel{}
+      )
+    ".
+
+  Definition prophet_wise_strong_snapshot γ past prophs : iProp Σ :=
+    prophet_wise_strong_full γ (past ++ prophs) ∗
+    mono_list_lb γ.(prophet_wise_strong_name_past) past.
+  #[local] Instance : CustomIpatFormat "snapshot" :=
+    " ( #Hfull{suff} &
+        #Hpast_lb
+      )
+    ".
+
+  Definition prophet_wise_strong_lb γ lb : iProp Σ :=
+    ∃ past,
+    prophet_wise_strong_snapshot γ past lb.
+  #[local] Instance : CustomIpatFormat "lb" :=
+    " ( %past{suff} &
+        Hsnapshot
+      )
+    ".
+
+  #[global] Instance prophet_wise_strong_full_timeless γ prophs :
+    Timeless (prophet_wise_strong_full γ prophs).
+  Proof.
+    apply _.
+  Qed.
+  #[global] Instance prophet_wise_strong_model_timeless pid γ past prophs :
+    Timeless (prophet_wise_strong_model pid γ past prophs).
+  Proof.
+    apply _.
+  Qed.
+  #[global] Instance prophet_wise_strong_snapshot_timeless γ past prophs :
+    Timeless (prophet_wise_strong_snapshot γ past prophs).
+  Proof.
+    apply _.
+  Qed.
+  #[global] Instance prophet_wise_strong_lb_timeless γ lb :
+    Timeless (prophet_wise_strong_lb γ lb).
+  Proof.
+    apply _.
+  Qed.
+
+  #[global] Instance prophet_wise_strong_full_persistent γ prophs :
+    Persistent (prophet_wise_strong_full γ prophs).
+  Proof.
+    apply _.
+  Qed.
+  #[global] Instance prophet_wise_strong_snapshot_persistent γ past prophs :
+    Persistent (prophet_wise_strong_snapshot γ past prophs).
+  Proof.
+    apply _.
+  Qed.
+  #[global] Instance prophet_wise_strong_lb_persistent γ lb :
+    Persistent (prophet_wise_strong_lb γ lb).
+  Proof.
+    apply _.
+  Qed.
+
+  Lemma prophet_wise_strong_model_exclusive pid γ1 past1 prophs1 γ2 past2 prophs2 :
+    prophet_wise_strong_model pid γ1 past1 prophs1 -∗
+    prophet_wise_strong_model pid γ2 past2 prophs2 -∗
+    False.
+  Proof.
+    iIntros "(:model =1) (:model =2)".
+    iApply (prophet_typed_strong_model_exclusive with "Hmodel1 Hmodel2").
+  Qed.
+
+  Lemma prophet_wise_strong_full_get pid γ past prophs :
+    prophet_wise_strong_model pid γ past prophs ⊢
+    prophet_wise_strong_full γ (past ++ prophs).
+  Proof.
+    iSteps.
+  Qed.
+  Lemma prophet_wise_strong_full_get' pid γ past prophs :
+    prophet_wise_strong_model pid γ past prophs ⊢
+      ∃ prophs',
+      prophet_wise_strong_full γ prophs'.
+  Proof.
+    rewrite prophet_wise_strong_full_get. iSteps.
+  Qed.
+  Lemma prophet_wise_strong_full_valid pid γ past prophs1 prophs2 :
+    prophet_wise_strong_model pid γ past prophs1 -∗
+    prophet_wise_strong_full γ prophs2 -∗
+    ⌜prophs2 = past ++ prophs1⌝.
+  Proof.
+    iIntros "(:model =1) (:full =2)".
+    iDestruct (agree_on_agree_L with "Hfull1 Hfull2") as %<-.
+    iSteps.
+  Qed.
+  Lemma prophet_wise_strong_full_agree γ prophs1 prophs2 :
+    prophet_wise_strong_full γ prophs1 -∗
+    prophet_wise_strong_full γ prophs2 -∗
+    ⌜prophs1 = prophs2⌝.
+  Proof.
+    apply agree_on_agree_L.
+  Qed.
+
+  Lemma prophet_wise_strong_snapshot_get pid γ past prophs :
+    prophet_wise_strong_model pid γ past prophs ⊢
+    prophet_wise_strong_snapshot γ past prophs.
+  Proof.
+    iIntros "(:model)".
+    iStep.
+    iApply (mono_list_lb_get with "Hpast_auth").
+  Qed.
+  Lemma prophet_wise_strong_snapshot_valid pid γ past1 prophs1 past2 prophs2 :
+    prophet_wise_strong_model pid γ past1 prophs1 -∗
+    prophet_wise_strong_snapshot γ past2 prophs2 -∗
+      ∃ past3,
+      ⌜past1 = past2 ++ past3⌝ ∗
+      ⌜prophs2 = past3 ++ prophs1⌝.
+  Proof.
+    iIntros "(:model) (:snapshot suff=')".
+    iDestruct (agree_on_agree_L with "Hfull Hfull'") as %Hfull.
+    iDestruct (mono_list_lb_valid with "Hpast_auth Hpast_lb") as %(past3 & ->).
+    iPureIntro. rewrite -assoc in Hfull. naive_solver.
+  Qed.
+
+  Lemma prophet_wise_strong_lb_get pid γ past prophs :
+    prophet_wise_strong_model pid γ past prophs ⊢
+    prophet_wise_strong_lb γ prophs.
+  Proof.
+    rewrite prophet_wise_strong_snapshot_get.
+    iSteps.
+  Qed.
+  Lemma prophet_wise_strong_lb_valid pid γ past prophs lb :
+    prophet_wise_strong_model pid γ past prophs -∗
+    prophet_wise_strong_lb γ lb -∗
+      ∃ past1 past2,
+      ⌜past = past1 ++ past2⌝ ∗
+      ⌜lb = past2 ++ prophs⌝.
+  Proof.
+    iIntros "Hmodel (:lb suff=')".
+    iExists past'.
+    iApply (prophet_wise_strong_snapshot_valid with "Hmodel Hsnapshot").
+  Qed.
+
+  Lemma prophet_wise_strong_wp_proph E :
+    {{{
+      True
+    }}}
+      Proph @ E
+    {{{ pid γ prophs,
+      RET #pid;
+      prophet_wise_strong_model pid γ [] prophs
+    }}}.
+  Proof.
+    iIntros "%Φ _ HΦ".
+    iApply wp_fupd. wp_apply (prophet_typed_strong_wp_proph with "[//]") as "%pid %prophs Hpid".
+    iMod (agree_alloc (agree_G := prophet_wise_strong_G_full_G) prophs) as "(%γ_full & #Hfull)".
+    iMod (mono_list_alloc []) as "(%γ_past & Hpast_auth)".
+    set γ := {|
+      prophet_wise_strong_name_full := γ_full ;
+      prophet_wise_strong_name_past := γ_past ;
+    |}.
+    iApply ("HΦ" $! pid γ).
+    iSteps.
+  Qed.
+
+  Lemma prophet_wise_strong_wp_resolve e pid v γ past prophs E Φ :
+    Atomic e →
+    to_val e = None →
+    prophet_wise_strong_model pid γ past prophs -∗
+    WP e @ E {{ w,
+      ∃ proph,
+      ⌜(w, v) = prophet.(prophet_typed_strong_to_val) proph⌝ ∗
+        ∀ prophs',
+        ⌜prophs = proph :: prophs'⌝ -∗
+        prophet_wise_strong_model pid γ (past ++ [proph]) prophs' -∗
+        Φ w
+    }} -∗
+    WP Resolve e #pid v @ E {{ Φ }}.
+  Proof.
+    iIntros "% % (:model) HΦ".
+    wp_apply (prophet_typed_strong_wp_resolve with "Hmodel"); first done.
+    iApply wp_fupd. wp_apply (wp_wand with "HΦ") as "%w (%proph & % & HΦ)".
+    iExists proph. iSplitR; first done.
+    iMod (mono_list_update_snoc proph with "Hpast_auth") as "Hpast_auth".
+    iIntros "!> %prophs' -> Hpid".
+    iApply ("HΦ" with "[//]").
+    rewrite (assoc _ _ [_]). iSteps.
+  Qed.
+End prophet_wise_G.
+
+#[global] Opaque prophet_wise_strong_full.
+#[global] Opaque prophet_wise_strong_model.
+#[global] Opaque prophet_wise_strong_snapshot.
+#[global] Opaque prophet_wise_strong_lb.
+
+Class ProphetWiseG Σ `{zoo_G : !ZooG Σ} prophet := {
+  #[local] prophet_wise_G :: ProphetWiseStrongG Σ prophet ;
+}.
+
+Definition prophet_wise_Σ prophet := #[
+  prophet_wise_strong_Σ prophet
+].
+#[global] Instance subG_prophet_wise_Σ Σ `{zoo_G : !ZooG Σ} prophet :
+  subG (prophet_wise_Σ prophet) Σ →
+  ProphetWiseG Σ prophet.
+Proof.
+  solve_inG.
+Qed.
+
+Section prophet_wise_G.
+  Context (prophet : prophet_typed).
+  Context `{prophet_wise_G : ProphetWiseG Σ prophet}.
+
+  Definition prophet_wise_name :=
+    prophet_wise_strong_name.
+  Implicit Types γ : prophet_wise_name.
+
+  Definition prophet_wise_full γ prophs : iProp Σ :=
+    ∃ sprophs,
+    ⌜prophs = sprophs.*2⌝ ∗
+    prophet_wise_strong_full prophet γ sprophs.
+  #[local] Instance : CustomIpatFormat "full" :=
+    " ( %sprophs{} &
+        -> &
+        Hfull{}
+      )
+    ".
+
+  Definition prophet_wise_model pid γ past prophs : iProp Σ :=
+    ∃ spast sprophs,
+    ⌜past = spast.*2⌝ ∗
+    ⌜prophs = sprophs.*2⌝ ∗
+    prophet_wise_strong_model prophet pid γ spast sprophs.
+  #[local] Instance : CustomIpatFormat "model" :=
+    " ( %spast{} &
+        %sprophs{} &
+        -> &
+        -> &
+        Hmodel{}
+      )
+    ".
+
+  Definition prophet_wise_snapshot γ past prophs : iProp Σ :=
+    ∃ spast sprophs,
+    ⌜past = spast.*2⌝ ∗
+    ⌜prophs = sprophs.*2⌝ ∗
+    prophet_wise_strong_snapshot prophet γ spast sprophs.
+  #[local] Instance : CustomIpatFormat "snapshot" :=
+    " ( %spast{} &
+        %sprophs{} &
+        -> &
+        -> &
+        Hsnapshot
+      )
+    ".
+
+  Definition prophet_wise_lb γ lb : iProp Σ :=
+    ∃ slb,
+    ⌜lb = slb.*2⌝ ∗
+    prophet_wise_strong_lb prophet γ slb.
+  #[local] Instance : CustomIpatFormat "lb" :=
+    " ( %slb &
+        -> &
+        Hlb
+      )
+    ".
+
+  #[global] Instance prophet_wise_full_timeless γ prophs :
+    Timeless (prophet_wise_full γ prophs).
+  Proof.
+    apply _.
+  Qed.
+  #[global] Instance prophet_wise_model_timeless pid γ past prophs :
+    Timeless (prophet_wise_model pid γ past prophs).
+  Proof.
+    apply _.
+  Qed.
+  #[global] Instance prophet_wise_snapshot_timeless γ past prophs :
+    Timeless (prophet_wise_snapshot γ past prophs).
+  Proof.
+    apply _.
+  Qed.
+  #[global] Instance prophet_wise_lb_timeless γ lb :
+    Timeless (prophet_wise_lb γ lb).
+  Proof.
+    apply _.
+  Qed.
+  #[global] Instance prophet_wise_full_persistent γ prophs :
+    Persistent (prophet_wise_full γ prophs).
+  Proof.
+    apply _.
+  Qed.
+  #[global] Instance prophet_wise_snapshot_persistent γ past prophs :
+    Persistent (prophet_wise_snapshot γ past prophs).
+  Proof.
+    apply _.
+  Qed.
+  #[global] Instance prophet_wise_lb_persistent γ lb :
+    Persistent (prophet_wise_lb γ lb).
+  Proof.
+    apply _.
+  Qed.
+
+  Lemma prophet_wise_model_exclusive pid γ1 past1 prophs1 γ2 past2 prophs2 :
+    prophet_wise_model pid γ1 past1 prophs1 -∗
+    prophet_wise_model pid γ2 past2 prophs2 -∗
+    False.
+  Proof.
+    iIntros "(:model =1) (:model =2)".
+    iApply (prophet_wise_strong_model_exclusive with "Hmodel1 Hmodel2").
+  Qed.
+
+  Lemma prophet_wise_full_get pid γ past prophs :
+    prophet_wise_model pid γ past prophs ⊢
+    prophet_wise_full γ (past ++ prophs).
+  Proof.
+    iIntros "(:model)".
+    rewrite -fmap_app. iSteps.
+    iApply (prophet_wise_strong_full_get with "Hmodel").
+  Qed.
+  Lemma prophet_wise_full_get' pid γ past prophs :
+    prophet_wise_model pid γ past prophs ⊢
+      ∃ prophs',
+      prophet_wise_full γ prophs'.
+  Proof.
+    rewrite prophet_wise_full_get. iSteps.
+  Qed.
+  Lemma prophet_wise_full_valid pid γ past prophs1 prophs2 :
+    prophet_wise_model pid γ past prophs1 -∗
+    prophet_wise_full γ prophs2 -∗
+    ⌜prophs2 = past ++ prophs1⌝.
+  Proof.
+    iIntros "(:model =1) (:full =2)".
+    iDestruct (prophet_wise_strong_full_valid with "Hmodel1 Hfull2") as %->.
+    list_simplifier. iSteps.
+  Qed.
+  Lemma prophet_wise_full_agree γ prophs1 prophs2 :
+    prophet_wise_full γ prophs1 -∗
+    prophet_wise_full γ prophs2 -∗
+    ⌜prophs1 = prophs2⌝.
+  Proof.
+    iIntros "(:full =1) (:full =2)".
+    iDestruct (prophet_wise_strong_full_agree with "Hfull1 Hfull2") as %->.
+    iSteps.
+  Qed.
+
+  Lemma prophet_wise_snapshot_get pid γ past prophs :
+    prophet_wise_model pid γ past prophs ⊢
+    prophet_wise_snapshot γ past prophs.
+  Proof.
+    iIntros "(:model)".
+    iSteps.
+    iApply (prophet_wise_strong_snapshot_get with "Hmodel").
+  Qed.
+  Lemma prophet_wise_snapshot_valid pid γ past1 prophs1 past2 prophs2 :
+    prophet_wise_model pid γ past1 prophs1 -∗
+    prophet_wise_snapshot γ past2 prophs2 -∗
+      ∃ past3,
+      ⌜past1 = past2 ++ past3⌝ ∗
+      ⌜prophs2 = past3 ++ prophs1⌝.
+  Proof.
+    iIntros "(:model) (:snapshot =')".
+    iDestruct (prophet_wise_strong_snapshot_valid with "Hmodel Hsnapshot") as "(%spast'' & -> & ->)".
+    list_simplifier. iSteps.
+  Qed.
+
+  Lemma prophet_wise_lb_get pid γ past prophs :
+    prophet_wise_model pid γ past prophs -∗
+    prophet_wise_lb γ prophs.
+  Proof.
+    iIntros "(:model)".
+    iStep.
+    iApply (prophet_wise_strong_lb_get with "Hmodel").
+  Qed.
+  Lemma prophet_wise_lb_valid pid γ past prophs lb :
+    prophet_wise_model pid γ past prophs -∗
+    prophet_wise_lb γ lb -∗
+      ∃ past1 past2,
+      ⌜past = past1 ++ past2⌝ ∗
+      ⌜lb = past2 ++ prophs⌝.
+  Proof.
+    iIntros "(:model) (:lb)".
+    iDestruct (prophet_wise_strong_lb_valid with "Hmodel Hlb") as "(%spast1 & %spast2 & -> & ->)".
+    list_simplifier. iSteps.
+  Qed.
+
+  Lemma prophet_wise_wp_proph E :
+    {{{
+      True
+    }}}
+      Proph @ E
+    {{{ pid γ prophs,
+      RET #pid;
+      prophet_wise_model pid γ [] prophs
+    }}}.
+  Proof.
+    iIntros "%Φ _ HΦ".
+    wp_apply (prophet_wise_strong_wp_proph prophet with "[//]") as "%pid %γ %sprophs Hmodel".
+    iApply "HΦ".
+    iExists [], sprophs. iSteps.
+  Qed.
+
+  Lemma prophet_wise_wp_resolve proph e pid v γ past prophs E Φ :
+    Atomic e →
+    to_val e = None →
+    v = prophet.(prophet_typed_to_val) proph →
+    prophet_wise_model pid γ past prophs -∗
+    WP e @ E {{ w,
+      ∀ prophs',
+      ⌜prophs = proph :: prophs'⌝ -∗
+      prophet_wise_model pid γ (past ++ [proph]) prophs' -∗
+      Φ w
+    }} -∗
+    WP Resolve e #pid v @ E {{ Φ }}.
+  Proof.
+    iIntros (? ? ->) "(:model) HΦ".
+    wp_apply (prophet_wise_strong_wp_resolve with "Hmodel"); first done.
+    wp_apply (wp_wand with "HΦ") as "%w HΦ".
+    iExists (w, proph). iStep. iIntros "%sprophs' -> Hmodel".
+    iApply ("HΦ" with "[//]").
+    iExists (spast ++ [(w, proph)]), sprophs'. iFrame.
+    list_simplifier. iSteps.
+  Qed.
+End prophet_wise_G.
+
+#[global] Opaque prophet_wise_name.
+#[global] Opaque prophet_wise_full.
+#[global] Opaque prophet_wise_model.
+#[global] Opaque prophet_wise_snapshot.
+#[global] Opaque prophet_wise_lb.
